Remove unnecessary imports and move definitions to pod_predicates.v and pvc_predicates.v

src/proof/controllers/statefulset/create_pvc.v
@@ -1,4 +1,4 @@
-From New.proof Require Import prelude empty_ffi.
+From New.proof.controllers.statefulset Require Export pod_predicates.
 From New.proof.controllers.statefulset Require Export pvc.
 From New.proof.kubernetes_model Require Export create_named_orphan get_reserved.
 From New.proof.map Require Import for_range.
@@ -42,80 +42,6 @@ Proof using package_sem.
 Defined.
 Context `{!kubernetesModelG Σ}.
 Local Set Default Proof Using "All".
-
-Definition new_persistent_volume_claim_key
-    (set : StatefulSetV.t) (claim_template : PersistentVolumeClaimV.t)
-    (ordinal : nat) : KKey.t :=
-  PersistentVolumeClaimV.key
-    (new_persistent_volume_claim set claim_template ordinal).
-
-Lemma new_persistent_volume_claim_key_eq set claim_template ordinal :
-  new_persistent_volume_claim_key set claim_template ordinal =
-    desired_pvc_key set
-      claim_template.(PersistentVolumeClaimV.ObjectMeta').(ObjectMetaV.Name')
-      ordinal.
-Proof.
-  unfold new_persistent_volume_claim_key, PersistentVolumeClaimV.key,
-    PersistentVolumeClaimV.meta_key, desired_pvc_key,
-    new_persistent_volume_claim.
-  done.
-Qed.
-
-Definition persistent_volume_claim_template_insert
-    (claim_templates : gmap go_string PersistentVolumeClaimV.t)
-    (claim_template : PersistentVolumeClaimV.t) :
-    gmap go_string PersistentVolumeClaimV.t :=
-  <[claim_template.(PersistentVolumeClaimV.ObjectMeta').(ObjectMetaV.Name') :=
-    claim_template]> claim_templates.
-
-Definition persistent_volume_claim_templates_by_name
-    (claim_templates : list PersistentVolumeClaimV.t) :
-    gmap go_string PersistentVolumeClaimV.t :=
-  fold_left persistent_volume_claim_template_insert claim_templates ∅.
-
-Lemma persistent_volume_claim_templates_by_name_snoc claim_templates
-    claim_template :
-  persistent_volume_claim_templates_by_name
-      (claim_templates ++ [claim_template]) =
-    persistent_volume_claim_template_insert
-      (persistent_volume_claim_templates_by_name claim_templates)
-      claim_template.
-Proof.
-  unfold persistent_volume_claim_templates_by_name.
-  by rewrite fold_left_app.
-Qed.
-
-Lemma persistent_volume_claim_templates_by_name_dom claim_templates :
-  dom (persistent_volume_claim_templates_by_name claim_templates) =
-    list_to_set
-      ((λ claim_template,
-          claim_template.(PersistentVolumeClaimV.ObjectMeta').(ObjectMetaV.Name'))
-        <$> claim_templates).
-Proof.
-  induction claim_templates using rev_ind.
-  - rewrite /persistent_volume_claim_templates_by_name /=
-      dom_empty_L. done.
-  - apply leibniz_equiv. apply set_equiv.
-    intros name.
-    assert (is_Some
-        (persistent_volume_claim_templates_by_name claim_templates !! name) ↔
-      name ∈ list_to_set (C:=gset go_string)
-        ((λ claim_template,
-            claim_template.(PersistentVolumeClaimV.ObjectMeta').(ObjectMetaV.Name'))
-          <$> claim_templates)) as Hprevious.
-    { rewrite -elem_of_dom IHclaim_templates. done. }
-    rewrite persistent_volume_claim_templates_by_name_snoc
-      /persistent_volume_claim_template_insert.
-    rewrite elem_of_dom lookup_insert_is_Some'.
-    rewrite fmap_app elem_of_list_to_set elem_of_app /=.
-    rewrite Hprevious elem_of_list_to_set.
-    rewrite list_elem_of_singleton.
-    split; intros [Hname|Hprevious'];
-      [right; symmetry; exact Hname
-      |left; exact Hprevious'
-      |right; exact Hname
-      |left; symmetry; exact Hprevious'].
-Qed.
 
 Definition claim_template_maps_related
     (R : v1.PersistentVolumeClaim.t → PersistentVolumeClaimV.t → Prop)
