src/proof/controllers/statefulset/pod_predicates.v
@@ -1,55 +1,262 @@
-From New.proof Require Import prelude empty_ffi.
-From New.proof.string Require Export prefix_suffix.
-From New.proof.kubernetes_model Require Export get index create delete.
-From New.proof Require Export util.
 From New.proof Require Export wp_helpers.
-From New.proof.controllers Require Export common.
-From New.proof.controllers.statefulset Require Export ordinal.
-From New.proof.controllers.statefulset Require Export pvc.
-From New.proof.controllers.statefulset Require Export statefulset_init.
-From New.proof.k8s_io.api.apps Require Export v1.
-From New.proof.k8s_io.kubernetes.pkg Require Export controller.
-From New.proof.k8s_io.apimachinery.pkg.runtime Require Export schema.
-From New.proof.k8s_io.apimachinery.pkg.api Require Export errors.
+From New.proof.string Require Export prefix_suffix.
+From New.proof.kubernetes_types Require Export prelude.
+From New.proof.controllers.statefulset Require Import pvc_predicates.
 
-Section proof.
-Context `{hG: !heapGS Σ} `{!ffi_semantics _ _}.
-Context {sem : go.Semantics}
-  {package_sem : code.controllers.statefulset.statefulset.Assumptions}.
-Collection W := sem + package_sem.
-#[local] Instance base_common_sem : common.Assumptions | 100 :=
-  code.controllers.statefulset.statefulset.import_common_Assumption.
-#[local] Instance controller_sem : controller.Assumptions :=
-  code.controllers.statefulset.statefulset.import_controller_Assumption.
-#[local] Instance runtime_sem : code.k8s_io.apimachinery.pkg.runtime.runtime.Assumptions :=
-  controller.import_runtime_Assumption.
-#[local] Instance runtime_object_underlying_eq :
-    runtime.Object ≤u runtime.Objectⁱᵐᵖˡ.
-Proof using package_sem. apply _. Qed.
-#[local] Instance meta_object_underlying_eq :
-    meta_v1.Object ≤u meta_v1.Objectⁱᵐᵖˡ.
-Proof using package_sem. apply _. Qed.
-#[local] Instance base_apimodel_sem : apimodel.Assumptions | 100 :=
-  common.import_apimodel_Assumption.
-#[local] Instance object_meta_v1_sem :
-    code.k8s_io.apimachinery.pkg.apis.meta.v1.v1.Assumptions :=
-  apimodel.import_apis_meta_v1_Assumption.
-#[local] Instance object_apps_v1_sem :
-    code.k8s_io.api.apps.v1.v1.Assumptions :=
-  apimodel.import_api_apps_v1_Assumption.
-#[local] Instance object_core_v1_sem :
-    code.k8s_io.api.core.v1.v1.Assumptions :=
-  code.k8s_io.api.apps.v1.v1.import_core_v1_Assumption.
-#[local] Instance apimodel_sem : apimodel.Assumptions | 0.
-Proof using package_sem.
-  constructor; try exact object_core_v1_sem; try apply _.
+Definition statefulset_replicas (sts : StatefulSetV.t) : nat :=
+  match sts.(StatefulSetV.Spec').(StatefulSetSpecV.Replicas') with
+  | Some replicas => sint.nat replicas
+  | None => 1%nat
+  end.
+
+Definition desired_ordinals (sts : StatefulSetV.t) : list nat :=
+  seq 0 (statefulset_replicas sts).
+
+Definition desired_pod_name (set_name : go_string) (ordinal : nat) : go_string :=
+  set_name ++ "-"%go ++ decimal_string ordinal.
+
+Definition desired_pod_key sts ordinal : KKey.t := {|
+  KKey.Kind' := PodV.kind;
+  KKey.Namespace' := sts.(StatefulSetV.ObjectMeta').(ObjectMetaV.Namespace');
+  KKey.Name' := desired_pod_name
+    sts.(StatefulSetV.ObjectMeta').(ObjectMetaV.Name') ordinal;
+|}.
+
+Definition desired_pod_keys (sts : StatefulSetV.t) : list KKey.t :=
+  desired_pod_key sts <$> desired_ordinals sts.
+
+Definition pod_key_is_desired (sts : StatefulSetV.t) (key : KKey.t) : Prop :=
+  key ∈ desired_pod_keys sts.
+
+#[global] Instance pod_key_is_desired_decision sts key :
+    Decision (pod_key_is_desired sts key).
+Proof. unfold pod_key_is_desired. apply _. Defined.
+
+Definition pod_has_member_name (set_name pod_name : go_string) : Prop :=
+  ∃ ordinal, pod_name = desired_pod_name set_name ordinal.
+
+Definition pod_has_member_key (sts : StatefulSetV.t) (pod : PodV.t) : Prop :=
+  ∃ ordinal, PodV.key pod = desired_pod_key sts ordinal.
+
+Lemma desired_pod_name_inj set_name ordinal1 ordinal2 :
+  desired_pod_name set_name ordinal1 = desired_pod_name set_name ordinal2 →
+  ordinal1 = ordinal2.
+Proof.
+  unfold desired_pod_name.
+  intros Hname.
+  apply app_inv_head in Hname.
+  inversion Hname as [Hdecimal].
+  by apply decimal_string_inj in Hdecimal.
+Qed.
+
+Lemma desired_pod_name_last_dash_decomp pod_name parent suffix set_name ordinal :
+  pod_name = parent ++ [byte_dash] ++ suffix →
+  byte_dash ∉ suffix →
+  pod_name = desired_pod_name set_name ordinal →
+  parent = set_name ∧ suffix = decimal_string ordinal.
+Proof.
+  intros Hdecomp Hsuffix_no_dash Hdesired.
+  rewrite Hdesired in Hdecomp.
+  unfold desired_pod_name in Hdecomp.
+  change "-"%go with [byte_dash] in Hdecomp.
+  eapply app_last_sep_inj in Hdecomp.
+  - destruct Hdecomp as [Hparent Hsuffix].
+    split; symmetry; done.
+  - apply decimal_string_dash_free.
+  - by apply dash_free_of_not_elem.
+Qed.
+
+Lemma desired_pod_name_has_dash set_name ordinal :
+  byte_dash ∈ desired_pod_name set_name ordinal.
+Proof.
+  unfold desired_pod_name.
+  change "-"%go with [byte_dash].
+  rewrite elem_of_app. right.
+  rewrite elem_of_app. left.
+  rewrite elem_of_cons. by left.
+Qed.
+
+Definition member_name_prefix (set_name : go_string) : go_string :=
+  set_name ++ "-"%go.
+
+Definition parse_member_name (set_name pod_name : go_string) : option nat :=
+  match New.proof.string.prefix_suffix.strip_prefix (member_name_prefix set_name)
+      pod_name with
+  | Some suffix => parse_canonical_decimal_string suffix
+  | None => None
+  end.
+
+Lemma parse_member_name_sound set_name pod_name ordinal :
+  parse_member_name set_name pod_name = Some ordinal →
+  pod_name = desired_pod_name set_name ordinal.
+Proof.
+  unfold parse_member_name.
+  destruct (New.proof.string.prefix_suffix.strip_prefix (member_name_prefix set_name)
+    pod_name) as [suffix|] eqn:Hstrip; [|done].
+  intros Hparse.
+  apply parse_canonical_decimal_string_sound in Hparse.
+  apply New.proof.string.prefix_suffix.strip_prefix_correct in Hstrip.
+  unfold desired_pod_name, member_name_prefix in *.
+  rewrite Hstrip.
+  rewrite -Hparse.
+  by rewrite List.app_assoc.
+Qed.
+
+Lemma parse_member_name_complete set_name pod_name ordinal :
+  pod_name = desired_pod_name set_name ordinal →
+  parse_member_name set_name pod_name = Some ordinal.
+Proof.
+  intros Hname.
+  unfold parse_member_name.
+  rewrite Hname.
+  unfold desired_pod_name, member_name_prefix.
+  rewrite List.app_assoc.
+  rewrite New.proof.string.prefix_suffix.strip_prefix_complete.
+  apply parse_canonical_decimal_string_decimal_string.
+Qed.
+
+#[global] Instance pod_has_member_name_decision set_name pod_name :
+  Decision (pod_has_member_name set_name pod_name).
+Proof.
+  destruct (parse_member_name set_name pod_name) as [ordinal|] eqn:Hparse.
+  - left. exists ordinal. by apply parse_member_name_sound.
+  - right. intros [ordinal Hname].
+    apply parse_member_name_complete in Hname.
+    congruence.
 Defined.
-#[local] Instance common_sem : common.Assumptions | 0.
-Proof using package_sem.
-  constructor; try exact apimodel_sem; try apply _.
+
+Definition pod_has_int32_member_name (set_name pod_name : go_string) : Prop :=
+  ∃ ordinal : nat,
+    (ordinal <= go_int32_max_nat)%nat ∧
+    pod_name = desired_pod_name set_name ordinal.
+
+#[global] Instance pod_has_int32_member_name_decision set_name pod_name :
+    Decision (pod_has_int32_member_name set_name pod_name).
+Proof.
+  unfold pod_has_int32_member_name.
+  destruct (parse_member_name set_name pod_name) as [ordinal|] eqn:Hparse.
+  - destruct (decide (ordinal <= go_int32_max_nat)%nat) as [Hbound|Hoverflow].
+    + left. exists ordinal. split; [done|].
+      by apply parse_member_name_sound.
+    + right. intros (ordinal' & Hbound & Hname).
+      apply parse_member_name_complete in Hname.
+      rewrite Hparse in Hname.
+      simplify_eq/=.
+      done.
+  - right. intros (ordinal & _ & Hname).
+    apply parse_member_name_complete in Hname.
+    congruence.
 Defined.
-Context `{!kubernetesModelG Σ}.
-Local Set Default Proof Using "All".
+
+Lemma pod_has_member_key_iff sts pod :
+  pod_has_member_key sts pod ↔
+  pod.(PodV.ObjectMeta').(ObjectMetaV.Namespace') =
+    sts.(StatefulSetV.ObjectMeta').(ObjectMetaV.Namespace') ∧
+  pod_has_member_name
+    sts.(StatefulSetV.ObjectMeta').(ObjectMetaV.Name')
+    pod.(PodV.ObjectMeta').(ObjectMetaV.Name').
+Proof.
+  split.
+  - intros [ordinal Hkey].
+    split.
+    + apply (f_equal KKey.Namespace') in Hkey. exact Hkey.
+    + exists ordinal.
+      apply (f_equal KKey.Name') in Hkey. exact Hkey.
+  - intros [Hnamespace [ordinal Hname]].
+    exists ordinal.
+    unfold PodV.key, PodV.meta_key, desired_pod_key.
+    simpl. by rewrite Hnamespace Hname.
+Qed.
+
+#[global] Instance pod_has_member_key_decision sts pod :
+  Decision (pod_has_member_key sts pod).
+Proof.
+  destruct (decide (
+    pod.(PodV.ObjectMeta').(ObjectMetaV.Namespace') =
+      sts.(StatefulSetV.ObjectMeta').(ObjectMetaV.Namespace') ∧
+    pod_has_member_name
+      sts.(StatefulSetV.ObjectMeta').(ObjectMetaV.Name')
+      pod.(PodV.ObjectMeta').(ObjectMetaV.Name'))) as [Hmember|Hnot_member].
+  - left. by apply pod_has_member_key_iff.
+  - right. intros Hmember_key.
+    apply Hnot_member. by apply pod_has_member_key_iff.
+Defined.
+
+Definition pod_ordinal_suffix (pod_name : go_string) : option go_string :=
+  match list_find (λ b, b = byte_dash) (reverse pod_name) with
+  | Some (idx, _) => Some (reverse (take idx (reverse pod_name)))
+  | None => None
+  end.
+
+Definition parse_pod_ordinal (pod_name : go_string) : option nat :=
+  suffix ← pod_ordinal_suffix pod_name;
+  parse_decimal_string suffix.
+
+Lemma pod_name_length_le_go_int_max_of_valid_name name :
+  valid_name PodV.kind name →
+  Z.of_nat (length name) ≤ go_int_max.
+Proof.
+  unfold valid_name, PodV.kind.
+  intros [[Hkind _]|([Hpod|[Hreplicaset|Hpvc]] & Hvalid_name)];
+    try discriminate.
+  destruct Hvalid_name as [_ Hlength].
+  unfold go_int_max. lia.
+Qed.
+
+Lemma pod_name_length_le_go_int_max_of_valid pod :
+  PodV.valid pod →
+  Z.of_nat
+    (length pod.(PodV.ObjectMeta').(ObjectMetaV.Name')) ≤ go_int_max.
+Proof.
+  intros (_ & _ & Hmeta & _).
+  apply pod_name_length_le_go_int_max_of_valid_name.
+  by apply ObjectMetaV.valid_name_of_valid.
+Qed.
+
+Lemma pod_name_length_le_go_int_max_of_valid_named_create namespace pod :
+  PodV.valid_named_create namespace pod →
+  Z.of_nat
+    (length pod.(PodV.ObjectMeta').(ObjectMetaV.Name')) ≤ go_int_max.
+Proof.
+  intros (_ & Hmeta & _).
+  apply pod_name_length_le_go_int_max_of_valid_name.
+  unfold ObjectMetaV.valid_named_create in Hmeta.
+  tauto.
+Qed.
+
+Example pod_has_member_name_accepts_one sts pod :
+  pod.(PodV.ObjectMeta').(ObjectMetaV.Name') =
+    sts.(StatefulSetV.ObjectMeta').(ObjectMetaV.Name') ++ "-1"%go →
+  pod_has_member_name
+    sts.(StatefulSetV.ObjectMeta').(ObjectMetaV.Name')
+    pod.(PodV.ObjectMeta').(ObjectMetaV.Name').
+Proof.
+  intros Hname.
+  exists 1%nat.
+  unfold desired_pod_name, decimal_string.
+  simpl.
+  exact Hname.
+Qed.
+
+Example pod_has_member_name_rejects_leading_zero sts pod :
+  pod.(PodV.ObjectMeta').(ObjectMetaV.Name') =
+    sts.(StatefulSetV.ObjectMeta').(ObjectMetaV.Name') ++ "-01"%go →
+  ¬ pod_has_member_name
+    sts.(StatefulSetV.ObjectMeta').(ObjectMetaV.Name')
+    pod.(PodV.ObjectMeta').(ObjectMetaV.Name').
+Proof.
+  intros Hname [ordinal Hmember].
+  pose proof (parse_member_name_complete
+    sts.(StatefulSetV.ObjectMeta').(ObjectMetaV.Name')
+    pod.(PodV.ObjectMeta').(ObjectMetaV.Name') ordinal Hmember) as Hparse.
+  unfold parse_member_name, member_name_prefix in Hparse.
+  rewrite Hname in Hparse.
+  replace (sts.(StatefulSetV.ObjectMeta').(ObjectMetaV.Name') ++ "-01"%go)
+    with ((sts.(StatefulSetV.ObjectMeta').(ObjectMetaV.Name') ++ "-"%go) ++
+      "01"%go) in Hparse by (rewrite -List.app_assoc; done).
+  rewrite New.proof.string.prefix_suffix.strip_prefix_complete in Hparse.
+  simpl in Hparse. done.
+Qed.
 
 Definition pod_identity_matches (sts : StatefulSetV.t) (pod : PodV.t) : Prop :=
   match parse_member_name
@@ -177,4 +384,19 @@ Definition pod_match (sts : StatefulSetV.t) (pod : PodV.t) : Prop :=
 #[global] Instance pod_match_decision sts pod : Decision (pod_match sts pod).
 Proof. unfold pod_match. apply _. Defined.
 
-End proof.
+Definition pod_is_condemned (set : StatefulSetV.t) (pod : PodV.t) : Prop :=
+  ∃ ordinal,
+    (ordinal ≤ go_int32_max_nat)%nat ∧
+    pod.(PodV.ObjectMeta').(ObjectMetaV.Name') =
+      desired_pod_name
+        set.(StatefulSetV.ObjectMeta').(ObjectMetaV.Name') ordinal ∧
+    (statefulset_replicas set ≤ ordinal)%nat.
+
+Definition pod_is_outdated (set : StatefulSetV.t) (pod : PodV.t) : Prop :=
+  ∃ ordinal,
+    (ordinal ≤ go_int32_max_nat)%nat ∧
+    pod.(PodV.ObjectMeta').(ObjectMetaV.Name') =
+      desired_pod_name
+        set.(StatefulSetV.ObjectMeta').(ObjectMetaV.Name') ordinal ∧
+    (ordinal < statefulset_replicas set)%nat ∧
+    ¬ pod_immutable_matches set pod.
